draft new version of rework
symbols as type, states as set
ignore invalid return values of the transition function (treat as Nop)
introduce type of valid tms
wrap the type in a "convenience" locale
define TM-specific consts and lemmas in the locale
to be continued

papers/116_stefan_rass/Supplementary/Lists.thy
@@ -1,7 +1,7 @@
 section\<open>Lists\<close>
 
 theory Lists
-  imports Main
+  imports Main Misc "HOL-Library.Sublist"
 begin
 
 text\<open>Extends \<^theory>\<open>HOL.List\<close>.\<close>
@@ -76,16 +76,19 @@ proof -
   then show "infinite X" using finite_maxlen by (rule contrapos_nn)
 qed
 
-abbreviation "pad n x xs \<equiv> xs @ x \<up> (n - length xs)"
+(* TODO this should be a definition *)
+abbreviation pad :: "nat \<Rightarrow> 'a \<Rightarrow> 'a list \<Rightarrow> 'a list"
+  where "pad n x xs \<equiv> xs @ x \<up> (n - length xs)"
 
-lemma pad_length: "length (pad n x xs) = max n (length xs)"
-  by simp
+lemma pad_length: "length (pad n x xs) = max n (length xs)" by simp
+lemma pad_le_length[simp]: "length xs \<le> n \<Longrightarrow> length (pad n x xs) = n" by simp
+lemma pad_ge_length[simp]: "length xs \<ge> n \<Longrightarrow> pad n x xs = xs" by simp
 
-lemma pad_le_length[simp]: "length xs \<le> n \<Longrightarrow> length (pad n x xs) = n"
-  by simp
+lemma pad_prefix: "prefix xs (pad n x xs)" by simp
 
 
 \<comment> \<open>\<open>ends_in\<close> - an alternative to \<^const>\<open>last\<close>.\<close>
+(* TODO this should be a definition *)
 abbreviation (input) ends_in :: "'a \<Rightarrow> 'a list \<Rightarrow> bool" where
   "ends_in x xs \<equiv> (\<exists>ys. xs = ys @ [x])"
 
@@ -226,5 +229,90 @@ next
   hence "set xs \<subseteq> {b}" by (rule trim_nil_set)
   with replicate_set_eq show "\<exists>n. xs = b \<up> n" ..
 qed
+
+
+text\<open>A version of \<^const>\<open>nth\<close> with a default value; if the requested element is not in the list,
+  the default value is returned instead.\<close>
+
+definition nth_or :: "nat \<Rightarrow> 'a \<Rightarrow> 'a list \<Rightarrow> 'a"
+  where "nth_or n x xs \<equiv> if n < length xs then xs ! n else x"
+
+lemma nth_or_simps:
+  shows nth_or_Nil: "nth_or n x [] = x"
+    and nth_or_val: "n < length xs \<Longrightarrow> nth_or n x xs = xs ! n"
+  unfolding nth_or_def by auto
+
+
+text\<open>Force a list to a given length; truncate if too long, and pad with the default value if too short.\<close>
+
+definition take_or :: "nat \<Rightarrow> 'a \<Rightarrow> 'a list \<Rightarrow> 'a list"
+  where "take_or n x xs \<equiv> pad n x (take n xs)"
+
+lemma take_or_length[simp]: "length (take_or n x xs) = n" unfolding take_or_def by force
+lemma take_or_id: "length xs = n \<Longrightarrow> take_or n x xs = xs" unfolding take_or_def by simp
+
+lemma take_or_altdef: "take_or n x xs = take n xs @ x \<up> (n - length xs)"
+proof (cases "length xs \<ge> n")
+  assume "length xs \<ge> n"
+  then have "length (take n xs) \<ge> n" by simp
+  with \<open>length xs \<ge> n\<close> show ?thesis unfolding take_or_def by force
+next
+  assume "\<not> length xs \<ge> n" hence "length xs < n" by simp
+  then have *: "take n xs = xs" by simp
+  show ?thesis unfolding take_or_def * ..
+qed
+
+
+text\<open>Force a list \<open>xs\<close> to match the length of another list \<open>ys\<close>;
+  truncate if \<open>xs\<close> is longer than \<open>ys\<close>, insert corresponding values from \<open>ys\<close> if \<open>xs\<close> is shorter.
+  Can also be interpreted as overwriting \<open>ys\<close> with values from \<open>xs\<close>;
+  if \<open>xs\<close> is longer the additional values are ignored,
+  if \<open>xs\<close> is shorter \<open>ys\<close> will retain some of its original values.\<close>
+
+(* TODO find a more intuitive name *)
+definition overwrite :: "'a list \<Rightarrow> 'a list \<Rightarrow> 'a list"
+  where "overwrite xs ys \<equiv> take (length ys) xs @ drop (length xs) ys"
+
+lemma overwrite_length: "length (overwrite xs ys) = length ys"
+proof -
+  let ?lx = "length xs" and ?ly = "length ys"
+  have "length (overwrite xs ys) = min ?lx ?ly + (?ly - ?lx)" unfolding overwrite_def by simp
+  also have "... = ?ly" by (cases "?ly \<ge> ?lx") auto
+  finally show ?thesis .
+qed
+
+lemma overwrite_id: "length xs = length ys \<Longrightarrow> overwrite xs ys = xs" unfolding overwrite_def by simp
+lemma overwrite_nth1: "n < min (length xs) (length ys) \<Longrightarrow> overwrite xs ys ! n = xs ! n"
+  unfolding overwrite_def nth_append by simp
+
+lemma overwrite_nth2:
+  assumes "n < length ys"
+    and "n \<ge> min (length xs) (length ys)"
+  shows "overwrite xs ys ! n = ys ! n"
+proof -
+  let ?lx = "length xs" and ?ly = "length ys"
+  from assms have "?lx \<le> ?ly" by linarith
+  then have lm: "min ?lx ?ly = ?lx" by force
+  then have lt: "length (take ?ly xs) = ?lx" by force
+  from \<open>n \<ge> min ?lx ?ly\<close> have "n \<ge> ?lx" unfolding lm .
+
+  from \<open>n \<ge> min ?lx ?ly\<close> have "\<not> n < length (take ?ly xs)" unfolding length_take by (rule leD)
+  then have "overwrite xs ys ! n = drop ?lx ys ! (n - ?lx)"
+    unfolding overwrite_def nth_append lt by presburger
+  also have "... = ys ! n" unfolding nth_drop[OF \<open>?lx \<le> ?ly\<close>] le_add_diff_inverse[OF \<open>n \<ge> ?lx\<close>] ..
+  finally show ?thesis .
+qed
+
+lemma overwrite_nth:
+  assumes "n < length ys" \<comment> \<open>to ensure there is a \<^const>\<open>nth\<close> element.\<close>
+  shows "overwrite xs ys ! n = (if n < min (length xs) (length ys) then xs ! n else ys ! n)"
+proof (rule ifI)
+  assume "n < min (length xs) (length ys)"
+  thus "overwrite xs ys ! n = xs ! n" by (rule overwrite_nth1)
+next
+  assume "\<not> n < min (length xs) (length ys)"
+  thus "overwrite xs ys ! n = ys ! n" by (intro overwrite_nth2[OF assms]) (rule leI)
+qed
+
 
 end
